src/lec2_sequences.dfy
@@ -1,0 +1,84 @@
+/* More interesting data to reason about: sequences. */
+
+/* In order to write proofs about interesting systems and protocols, we first
+need some way of modeling the state of those systems and protocols. We'll
+explore Dafy's built-in sequence type as well as algebraic data types, its core
+way of creating user-defined types. */
+
+/*** Sequences ***/
+
+/* These data types are very similar to data structures, but will be purely
+ * mathematical. We'll start with the sequence type `seq<T>`. The `T` in angle
+ * brackets is a _type parameter_, needed because sequences can hold values of
+ * any type. A sequence is related to data structures you're familiar with like
+ * linked lists or arrays/vectors (the terminology depends on the programming
+ * language). A sequence is the mathematical essence of the state of a
+ * list/vector/array without the implementation details.
+ */
+
+lemma SequenceOperations()
+{
+  // var is a (mutable) local variable, defined within a lemma
+  var s: seq<int> := [3, 1, 2];
+  // sequences can be indexed, starting at 1
+  assert s[1] == 1;
+  // we can extract a subsequence
+  assert s[1..2] == [1];
+  // we can re-assign the sequence and update one element using the `s[i := v]` syntax.
+  s := s[2 := 3];
+  assert s[0] == s[2] == 3;
+  // `|s|` is the sequence's length
+  assert |s| == 3;
+  // we can append two sequences
+  s := s + [7, 12];
+  assert |s| == 5;
+  assert s == [3, 1, 3, 7, 12];
+}
+
+/* Below we give some lemmas illustrating sequence operations. */
+
+function SeqGet(s: seq<int>, i: nat): int
+  // New feature (function preconditions): functions can have _requires_
+  // clauses, also called _preconditions_. Dafny will statically check  that the
+  // preconditions hold (in the same way as assertions) wherever a call to the
+  // function appears.
+  //
+  // This particular precondition requires that the index is in-bounds. The fact
+  // that `i` is of type `nat` already assures that it is non-negative.
+  requires i < |s|
+{
+  s[i]
+}
+
+function SeqUpdate(s: seq<int>, i: nat, n: int): seq<int>
+  requires i < |s|
+{
+  s[i := n]
+}
+
+lemma CheckedPreconditions(s: seq<int>, i: nat)
+  // Dafny does not allow even stating this because it tries to index a //
+  // sequence without a proof that the index is in-bounds, one of the preconditions
+  // for sequence indexing.
+  //
+  // We'd get the same error in an ensures clause or function definition.
+  requires s[i] > 0 // error: index out of range
+{}
+
+lemma CheckedFunctionPreconditions(s: seq<int>, i: nat)
+  // almost same as above, but notice that the error specifically points to the
+  // `SeqGet` precondition
+  requires SeqGet(s, i) > 0 // error: function precondition might not hold
+{}
+
+lemma SequenceAppendFact(s1: seq<int>, s2: seq<int>)
+  // New feature (forall where clause): notice the new pipe symbol after the `i`.
+  // The general syntax is of the form `forall x | p(x) :: q(x)`; it means the
+  // same thing as `forall x :: p(x) ==> q(x)` but can be easier to read. You
+  // might read this as "for all x where p(x), q(x)".
+  //
+  // We're also leaving off the type of `i` because Dafny can infer that it's an `int`.
+  ensures forall i | |s1| <= i < |s1| + |s2| :: (s1 + s2)[i] == s2[i - |s1|]
+{
+  // goes through without any extra proof
+}
